dataplane/Correctness/Produces.thy
@@ -1,0 +1,223 @@
+theory Produces
+
+imports
+  General
+  Dataplane.Timely_Stream
+  Dataplane.MyProduct_Instances
+  Dataplane.AntichainOrder
+begin
+
+declare cin.rep_eq[simp del]
+declare enum_class.enum_UNIV[simp] enum_class.enum_distinct[simp]
+no_notation shiftr  (infixl \<open>>>\<close> 55)
+
+
+find_theorems filter zmset
+
+(*
+   (\<forall> p. to_zmset (drops p) \<subseteq>#\<^sub>z zmset (map snd (filter (\<lambda>x. p = fst x) produs))) \<Longrightarrow>
+*)
+
+(* FIXME: move me *)
+lemma to_zmset_list_diff[simp]:
+  "mset ys \<subseteq># mset xs \<Longrightarrow>
+   to_zmset (list_diff xs ys) = to_zmset xs - to_zmset ys"
+  apply (induct xs ys rule: list_diff.induct)
+   apply clarsimp+
+  apply (metis add_zmset_diff_bothsides insert_DiffM insert_subset_eq_iff mset_remove_last to_zmset_correct zmset_of_add_mset)
+  done
+
+lemma outputs_at_target_updates[simp]:
+  "outputs_at_target su (os(nid := (os nid)\<lparr> inter := A \<rparr>)) = outputs_at_target su os"
+  "outputs_at_target su (os(nid := (os nid)\<lparr> produ := B \<rparr>)) = outputs_at_target su os"
+  "outputs_at_target su (os(nid := (os nid)\<lparr> ocaps := C \<rparr>)) = outputs_at_target su os"
+  "outputs_at_target su (os(nid := (os nid)\<lparr> input := D \<rparr>)) = outputs_at_target su os"
+  "outputs_at_target su (os(nid := (os nid)\<lparr> inter := E \<rparr>)) = outputs_at_target su os"
+  "outputs_at_target su (os(nid := (os nid)\<lparr> nfron := F \<rparr>)) = outputs_at_target su os"
+  unfolding outputs_at_target_def
+  apply (rule ext)
+  apply (auto split: prod.splits if_splits)
+  done
+
+
+
+lemma to_zmset_BULK_BENQ[simp]:
+  "to_zmset ((xs >> ys) p) = to_zmset (xs p) + to_zmset (ys p)"
+  unfolding BULK_BENQ_def
+  by auto
+
+lemma find_Some_singleton:
+  "{x \<in> set xs . P x} = {x} \<Longrightarrow>
+   find P xs = Some x"
+  apply (induct xs)
+  apply simp_all
+  apply (auto 0 0 simp add:)
+   apply blast
+  apply (smt (verit, best) Collect_cong)
+  done
+
+find_consts  "('a \<times> 'b) set \<Rightarrow> bool" name: inj
+
+(* 
+lemma graph_to_nxt_Src_from_Trg:
+  "(\<forall> nid p. card (Src_from_Trg su nid p) \<le> 1) \<Longrightarrow>
+   (\<forall> nid p. card (Trg_from_Src su nid p) \<le> 1) \<Longrightarrow>
+   graph_to_nxt su ((nid' :: 'nid :: enum), (p' :: 'p :: enum)) = Some (nid :: 'nid, p :: 'p) \<longleftrightarrow> Src_from_Trg su nid p = {(nid', p' :: 'p)}"
+  unfolding graph_to_nxt_def Src_from_Trg_def
+  apply (auto simp add: card_eq_Suc_0_ex1 le_eq_less_or_eq)
+  subgoal for nid p
+    by (metis (mono_tags, lifting) find_SomeD(1) is_empty_antichain_simp old.prod.case old.prod.inject)
+ *)
+
+lemma eq_singletonD:
+  "{x. P x} = {x} \<Longrightarrow> P x"
+  by auto
+
+lemma in_op_conn_graph_to_nxt_iff:
+  "single_valued (op_conn su) \<Longrightarrow>
+   graph_to_nxt su (nid, p) = Some (nid', p') \<longleftrightarrow> ((nid, p), nid', p') \<in> op_conn su"
+  unfolding graph_to_nxt_def op_conn_def
+  apply (auto simp add: is_empty_antichain_iff split: prod.splits)
+  subgoal
+    apply (auto simp add: single_valued_def dest!: find_SomeD' split: prod.splits)
+    done
+  subgoal
+    apply (rule find_Some_singleton)
+    apply (auto simp add: single_valued_def split: prod.splits)
+    done
+  done
+
+lemma graph_to_nxt_not_Ex_op_conn[simp]:
+  "graph_to_nxt su (nid, p) = None \<longleftrightarrow>
+   \<not> (\<exists> nid' p'. ((nid, p), nid', p') \<in> op_conn su)"
+  unfolding graph_to_nxt_def op_conn_def
+  apply (auto simp add: is_empty_antichain_iff find_None_iff dest!: find_SomeD' split: prod.splits)
+  done
+
+lemma
+    "outputs_at_target su (os((nid :: 'n :: enum) := (os nid)\<lparr> outpu := (\<lambda>(p :: 'p). oputs p) \<rparr>)) (nid', p') =
+     (let S = {p''. su (Loc nid (Src p'')) (Loc nid' (Trg p')) \<noteq> {}\<^sub>A} in if S \<noteq> {} then oputs (Set.the_elem S) else outputs_at_target su os (nid', p'))"
+  unfolding outputs_at_target_def
+  apply (clarsimp split: prod.splits if_splits)
+  subgoal for a
+    unfolding  le_eq_less_or_eq
+    apply (auto simp add: card_eq_0_iff card_1_singleton_iff)
+    subgoal for p nid'
+      apply hypsubst_thin
+      apply (rule FalseE)
+      oops
+
+lemma
+  "single_valued ((op_conn su)\<inverse>) \<Longrightarrow>
+   summ sg (Loc nid'' (Src p'')) (Loc nid' (Trg p')) \<noteq> {}\<^sub>A \<Longrightarrow>
+   the_elem {(nid'', p''). ((nid'', p''), nid', p') \<in> op_conn (summ sg)} = (nid, p) \<Longrightarrow>
+   ((nid, p), nid', p') \<in> op_conn su"
+  unfolding graph_to_nxt_def op_conn_def the_elem_def
+  apply (auto simp add: single_valued_def dest!: split: prod.splits)
+  subgoal
+    oops
+
+
+lemma dataplane_tracker_inv_produces_drops:
+  fixes drops :: "'p :: {enum,linorder} \<Rightarrow> 't :: {ccompare,canonically_ordered_monoid_add,ordered_ab_semigroup_monoid_add_imp_le,bot} list"
+  shows
+    "noutput = (\<lambda> p . outpu (os nid) p @ oputs p) \<Longrightarrow>
+   nocaps = (\<lambda> p . list_diff (ocaps (os nid) p) (drops p)) \<Longrightarrow>
+   ninput = (\<lambda> p. filter (\<lambda> (_, t). t \<notin> set (drops p)) (input (os nid) p)) \<Longrightarrow> 
+   nprodu = produ (os nid) @ produs \<Longrightarrow>
+   ninter = operator_state.inter (os nid) @ concat (map (\<lambda> p. map (\<lambda>os. (p, os, - 1)) (drops p)) Enum.enum) \<Longrightarrow>
+   (\<forall> p. mset (drops p) \<subseteq># mset (ocaps (os nid) p)) \<Longrightarrow>
+   (\<forall> (p, t, m) \<in> set produs. m > 0 \<and> t \<in> set (ocaps (os nid) p)) \<Longrightarrow>
+   (\<forall> p. snd ` set (oputs p) \<subseteq> set (ocaps (os nid) p)) \<Longrightarrow>
+   (\<forall> p. to_zmset (map snd (oputs p)) = zmset (map snd (filter (\<lambda>x. p = fst x) produs))) \<Longrightarrow>
+   graph_summar_nt (summ sg) (nxt sg) os \<Longrightarrow>
+   nxt sg = graph_to_nxt (summ sg) \<Longrightarrow>
+   dataplane_tracker_inv os cbufs sg \<Longrightarrow>
+   dataplane_tracker_inv (os(nid := os nid \<lparr>outpu := noutput, ocaps := nocaps, input := ninput, produ := nprodu, inter := ninter, nfron := V\<rparr>)) cbufs sg"
+  unfolding dataplane_tracker_inv_def
+  apply (elim conjE exE)
+  apply simp
+  apply hypsubst_thin
+  subgoal premises temp for c c' cgs chns caps
+    using temp(5)[unfolded graph_summar_nt_def] apply -
+    apply clarsimp
+    subgoal premises GS
+      using temp(1,2,3,4,6-) apply-
+      apply (rule exI[of _ 
+            "(\<lambda> l. case l of 
+       Loc nid' (Src p') \<Rightarrow> if nid' = nid then caps l - to_zmset (drops p') else caps l 
+     | Loc nid' (Trg p') \<Rightarrow>  caps l + zmset (map snd (filter (\<lambda> (p'', _, _). (graph_to_nxt (summ sg)) (nid, p'') = Some (nid', p')) produs)))"])
+      apply (intro conjI)
+      subgoal premises prems
+        using prems(6)
+        unfolding Src_caps_inv_def
+        by (auto simp add: temp(1))
+      subgoal premises prems
+        using prems(7,8) apply -
+        unfolding Trg_caps_inv_def
+        apply (clarsimp simp add: to_zmset_map)
+        subgoal for nid' p'
+          apply (drule spec[of _ nid'])
+          apply (drule spec[of _ p'])
+          unfolding c_pts_inv_def
+          apply (drule spec[of _ "Loc nid' (Trg p')"])
+          apply (drule sym)
+          back
+          apply simp
+          apply (auto simp add: in_op_conn_graph_to_nxt_iff[OF GS(7)] outputs_at_target_def split: prod.splits if_splits)
+          subgoal for nid'' p''' p''
+            apply (subst temp(4)[rule_format, of p''', unfolded to_zmset_map, simplified])
+            apply (rule arg_cong[where f=zmset])
+            apply (rule map_cong)
+            subgoal
+              apply (rule filter_cong)
+               apply (auto split: prod.splits simp add: op_conn_def )
+              subgoal
+                apply (drule GS(8)[unfolded op_conn_def single_valued_def, simplified, rule_format])
+                 apply assumption
+                apply auto
+                apply hypsubst_thin
+                apply (subst (asm) the_elem_image_unique[where f=id, simplified])
+                  apply blast
+                 apply clarsimp
+                using GS(8)[unfolded op_conn_def single_valued_def, simplified, rule_format] apply blast
+                apply auto
+                done
+              subgoal
+                apply (subst (asm) the_elem_image_unique[where f=id, simplified])
+                  apply blast
+                 apply clarsimp
+                using GS(8)[unfolded op_conn_def single_valued_def, simplified, rule_format] apply blast
+                apply auto
+                done
+              done
+            apply simp
+            done
+          subgoal
+            apply (subst filter_False)
+             apply simp_all
+            subgoal
+              apply (auto split: prod.splits simp add: op_conn_def )
+              apply (subst (asm) the_elem_image_unique[where f=id, simplified])
+                apply blast
+               apply clarsimp
+              using GS(8)[unfolded op_conn_def single_valued_def, simplified, rule_format] apply blast+
+              done
+            done
+          done
+        done
+      subgoal premises prems
+        using prems(8) apply -
+        unfolding c_pts_inv_def
+        apply safe
+        subgoal for l
+          apply (drule spec[of _ l])
+          apply (drule sym)
+          apply (auto simp add:  c_pts_change_multiplicities split: location.splits port.splits; hypsubst_thin)
+          subgoal for nid' p'
+          
+
+
+
+
+end
